Dafny/Resolver.cs
@@ -103,7 +103,6 @@ namespace Microsoft.Dafny {
     [ContractInvariantMethod]
     void ObjectInvariant() {
       Contract.Invariant(builtIns != null);
-      Contract.Invariant(cce.NonNullDictionaryAndValues(classes));
       Contract.Invariant(cce.NonNullElements(importGraph));
       Contract.Invariant(cce.NonNullDictionaryAndValues(classMembers) && Contract.ForAll(classMembers.Values, v => cce.NonNullDictionaryAndValues(v)));
       Contract.Invariant(cce.NonNullDictionaryAndValues(datatypeCtors) && Contract.ForAll(datatypeCtors.Values, v => cce.NonNullDictionaryAndValues(v)));
